Cslib/Logics/Propositional/Defs.lean
@@ -6,10 +6,7 @@ Authors: Thomas Waring
 
 module
 
-public import Cslib.Foundations.Logic.Operators.And
-public import Cslib.Foundations.Logic.Operators.Or
-public import Cslib.Foundations.Logic.Operators.Impl
-public import Cslib.Foundations.Logic.Operators.Not
+public import Cslib.Foundations.Logic.Operators
 public import Cslib.Foundations.Logic.InferenceSystem
 public import Mathlib.Data.FunLike.Basic
 public import Mathlib.Data.Set.Image
@@ -57,25 +54,25 @@ inductive Proposition (Atom : Type u) : Type u where
   /-- Disjunction -/
   | or (a b : Proposition Atom)
   /-- Implication -/
-  | impl (a b : Proposition Atom)
+  | imp (a b : Proposition Atom)
 deriving DecidableEq, BEq
 
 instance instBotProposition [Bot Atom] : Bot (Proposition Atom) := ⟨.atom ⊥⟩
 instance instInhabitedOfBot [Bot Atom] : Inhabited Atom := ⟨⊥⟩
 
 /-- We view negation as a defined connective ~A := A → ⊥ -/
-abbrev Proposition.neg [Bot Atom] : Proposition Atom → Proposition Atom := (Proposition.impl · ⊥)
+abbrev Proposition.neg [Bot Atom] : Proposition Atom → Proposition Atom := (Proposition.imp · ⊥)
 
 /-- A fixed choice of a derivable proposition (of course any two are equivalent). -/
-abbrev Proposition.top [Inhabited Atom] : Proposition Atom := impl (.atom default) (.atom default)
+abbrev Proposition.top [Inhabited Atom] : Proposition Atom := imp (.atom default) (.atom default)
 
 instance instTopProposition [Inhabited Atom] : Top (Proposition Atom) := ⟨.top⟩
 
-example [Bot Atom] : (⊤ : Proposition Atom) = Proposition.impl ⊥ ⊥ := rfl
+example [Bot Atom] : (⊤ : Proposition Atom) = Proposition.imp ⊥ ⊥ := rfl
 
 instance : HasAnd (Proposition Atom) := {and := Proposition.and}
 instance : HasOr (Proposition Atom) := {or := Proposition.or}
-instance : HasImpl (Proposition Atom) := {impl := Proposition.impl}
+instance : HasImp (Proposition Atom) := {imp := Proposition.imp}
 instance [Bot Atom] : HasNot (Proposition Atom) := {not := Proposition.neg}
 
 omit [DecidableEq Atom] in
@@ -89,7 +86,7 @@ def Proposition.subst {Atom Atom' : Type u} (f : Atom → Proposition Atom') :
   | atom x => f x
   | and A B => (A.subst f) ∧ (B.subst f)
   | or A B => (A.subst f) ∨ (B.subst f)
-  | impl A B => (A.subst f) → (B.subst f)
+  | imp A B => (A.subst f) → (B.subst f)
 
 -- This is probably a lawful monad, but that doesn't seem to be important.
 instance : Monad Proposition where
